TM/Code/WriteValue.v
@@ -1,6 +1,7 @@
 Require Import CodeTM.
 Require Import TM.Basic.WriteString.
 Require Import Basic.Mono.
+Require Import TMTac.
 
 
 Lemma WriteString_L_right (sig : Type) (str : list sig) t :
